protocol updated to match processings algotithms in report

Protocol/SAMLProtocol.fst
@@ -3,40 +3,55 @@ module SamlProtocol
 open Crypto
 (*open Network*)
 
-
-type AuthnRequest = {id:string;  
-                    IssueInstant:string;     
-                    Destination:endpoint;
-                    Issuer:prin}
-
-
 type assertiontoken = string (*Add refinements*)
 type signedtoken = string (*Add refinements*)
 type id = string
 type endpoint = string
 type uri = string
 
+type AuthnRequest = 
+  | MkAuthnRequest: id:string ->
+                    IssueInstant:string ->
+                    Destination:endpoint ->
+                    Issuer:prin ->
+                    message:string ->
+                    sig:dsig ->
+                    AuthnRequest
+
+type LoginData = 
+  | MkLoginData:  user:prin ->
+                  signature:dsig ->
+                  cert:pubkey user ->
+                  challenge:nonce ->
+                  site:string -> 
+                  data:string ->
+                  LoginData
+
 type Assertion =
   | SignedAssertion: assertiontoken -> dsig -> Assertion
-  | EncryptedAssertion: encrypter:prin -> prinencryptedtoken:string -> Assertion
-
-type SamlMessage =
-  | Login: uri -> SamlMessage
-  | LoginResponse: string -> SamlMessage
-  | AuthnRequest: issuer:prin ->  destination:endpoint -> message:string -> dsig -> SamlMessage
-  | AuthResponseMessage: issuer:prin -> destination:endpoint -> Assertion -> SamlMessage
-  | UserCredRequest: challenge:nonce -> SamlMessage
-  | Failed: int -> SamlMessage
+  | EncryptedAssertion: cypher -> Assertion
 
 type SamlStatus =
   | Success: SamlStatus
   | Requester: SamlStatus
   | Responder: SamlStatus
 
+type SamlMessage =
+  | Login: uri -> SamlMessage
+  | LoginResponse: string -> SamlMessage
+  | AuthnRequestMessage: issuer:prin ->  destination:endpoint -> message:string -> dsig -> SamlMessage
+  | AuthResponseMessage: issuer:prin -> destination:endpoint -> Assertion -> SamlMessage
+  | UserAuthenticated: status:string -> loginData:LoginData -> authnRequest:AuthnRequest -> SamlMessage
+  | UserCredRequest: challenge:nonce -> SamlMessage
+  | Failed: SamlStatus -> SamlMessage
+  | DisplayError: int -> SamlMessage
+
 
 val SendSaml: prin -> SamlMessage -> unit
 val ReceiveSaml: prin -> SamlMessage 
 
-val IssuerAssertion: issuer:prin -> subject:prin -> audience:prin -> inresto:id -> assertiontoken
-val AddSignatureToAssertion: assertiontoken -> dsig -> signedtoken
 val CreateAuthnRequestMessage: issuer:prin -> destination:prin -> string
+val IssueAssertion: issuer:prin -> subject:prin -> audience:prin -> inresto:id -> assertiontoken
+val AddSignatureToAssertion: assertiontoken -> dsig -> signedtoken
+val EncryptAssertion: receiver:prin -> pubkey receiver -> signedtoken -> Assertion
+val DecryptAssertion: receiver:prin -> privkey receiver -> Assertion -> (signedtoken * dsig)
