Protocol/ServiceProvider.fst
@@ -3,30 +3,31 @@ module Serviceprovider
 open SamlProtocol
 open Crypto
 
-
-
-val serviceprovider:  me:prin -> pubkey me -> privkey me ->
-                      client:prin -> idp:prin -> pubkey idp -> unit 
-let serviceprovider me pubk privk client idp pubkidp = 
+val serviceprovider:  me:prin -> client:prin -> idp:prin -> unit 
+let rec serviceprovider me client idp = 
  let req = ReceiveSaml client in
  match req with
   | Login (url) -> (*Create AuthnRequest and send back*)
     let authnReq = CreateAuthnRequestMessage me idp in
     assume(Log me authnReq) (*Protocol event*);
-    let sigSP = Sign me privk authnReq in
-    let resp = AuthnRequest me idp authnReq sigSP in 
+    let myprivk = CertStore.GetPrivateKey me in
+    let sigSP = Sign me myprivk authnReq in
+    let resp = AuthnRequestMessage me idp authnReq sigSP in 
     SendSaml client resp; (*2*)
-    serviceprovider me pubk privk client idp pubkidp (*Start over*)
+    serviceprovider me client idp (*Start over*)
 
-  | AuthResponseMessage (issuer, destination, assertion) -> 
+  | AuthResponseMessage (issuer, destination, encassertion) -> 
+    let myprivk = CertStore.GetPrivateKey me in
+    let assertion = DecryptAssertion me myprivk encassertion in
     match assertion with
     | SignedAssertion (token,sigIDP) ->
-      if VerifySignature idp pubkidp token sigIDP
+      let pubkissuer = CertStore.GetPublicKey idp in
+      if VerifySignature idp pubkissuer token sigIDP
       then
         (assert(Log idp token);
         let resp = LoginResponse "You are now logged in" in
-        SendSaml client resp) (*8*)
-      else SendSaml client (Failed 403);(*8.1*)
-      serviceprovider me pubk privk client idp pubkidp (*Start over*)
-  | _ -> SendSaml client (Failed 400);(*8.1*)
-        serviceprovider me pubk privk client idp pubkidp (*Start over*)
+        SendSaml client resp) (*12*)
+      else SendSaml client (DisplayError 403);(*12.1*)
+      serviceprovider me client idp (*Start over*)
+  | _ -> SendSaml client (DisplayError 400);(*2.1*)
+        serviceprovider me client idp (*Start over*)
