Protocol/Crypto.fst
@@ -5,16 +5,16 @@ type prin = string
 type pubkey :: prin => *
 type privkey :: prin => *
 type dsig
-type nonce
+type nonce = string
 type cypher
 
 (*Verification*)
 type Log :: prin => string => E
 
-val Keygen:  p:prin
+val Keygen: p:prin
           -> (pubkey p * privkey p)
 
-val Sign:  p:prin
+val Sign: p:prin
         -> privkey p
         -> msg:string{Log p msg}
         -> dsig
@@ -25,16 +25,15 @@ val VerifySignature: p:prin
         -> dsig
         -> b:bool{b=true ==> Log p msg}
 
-
 val Encrypt: p:prin
         -> pubkey p
-        -> msg:string{Log p msg}
+        -> string
         -> cypher
 
 val Decrypt: p:prin
-        -> p privkey
+        -> privkey p
         -> cypher
-        -> msg:string
+        -> string
 
 val GenerateNonce: prin -> nonce (*Add refinement to ensure unqueness*)
 
@@ -42,14 +41,3 @@ val AuthenticateUser: user:string
         -> password:string
         -> challenge:nonce 
         -> b:bool{b=true ==> Log user challenge}
-
-
-(*Crypto functions*)
-extern reference Crypto {language="F#";
-            dll="Crypto";
-            namespace="";
-            classname="Crypto"}
-
-extern Crypto val KeyGenExt: p:prin
-          -> (string * string)
-
