Protocol/certstore.fst
@@ -1,0 +1,8 @@
+module CertStore
+
+open Crypto
+
+val GetPublicKey: p:prin -> pubkey p
+
+(*Prin needs to include credentials*)
+val GetPrivateKey: p:prin -> privkey p 
