Protocol/httpprotocol.fst
@@ -1,0 +1,6 @@
+module HttpProtocol
+
+type HttpMessage =
+  | Get: uri -> HttpMessage
+  | Post: uri -> HttpMessage
+  | Redirect: destination -> message -> HttpMessage
