Protocol/main.fst
@@ -11,5 +11,5 @@ let main attacker =
 	let sppk, spsk = Keygen "https://serviceprovider.org" in 
 	let idppk, idpsk = Keygen "https://identityprovider.org" in 
 	Fork [	attacker;
-		(fun () -> serviceprovider "https://serviceprovider.org" sppk spsk "browser" "https://identityprovider.org" idppk);
-		(fun () -> identityprovider "https://identityprovider.org" idppk idpsk "browser" "https://serviceprovider.org" sppk)]
+		(fun () -> serviceprovider "https://serviceprovider.org" "browser" "https://identityprovider.org");
+		(fun () -> identityprovider "https://identityprovider.org" "browser")]
