Protocol/report-examples/sum.fst
@@ -1,0 +1,6 @@
+module Sum
+
+val sum: int -> int -> int
+let sum x y = x+y
+
+let tree = sum 1 2
