Protocol/samltypes.fst
@@ -1,0 +1,6 @@
+module samltypes
+
+type AuthnRequest = {id:string;  
+                    IssueInstant:string;     
+                    Destination:endpoint;
+                    Issuer:prin}
